More diagramatic reasoning

examples/Imp2AsmBis.v
@@ -1,17 +1,38 @@
-From ITree Require Import ITree.
+
+From Coq Require Import
+     Program
+     Lia
+     Setoid
+     Morphisms
+     RelationClasses.
+
+
+From ITree Require Import ITree FixFacts.
 
 Require Import Program.Basics. (* ∘ *)
+
+  Set Nested Proofs Allowed.
 
 (* Diagramatic/categorical sum combinators. *)
 
 Definition id {A} (x : A) : A := x.
 
-Definition sum_bimap {A B C D} (f : A -> B) (g : C -> D)
-           (ac : A + C) : B + D :=
-  match ac with
-  | inl a => inl (f a)
-  | inr c => inr (g c)
-  end.
+Definition sum_elim {A B C} (f : A -> C) (g : B -> C) : A + B -> C :=
+  fun x =>
+    match x with
+    | inl a => f a
+    | inr b => g b
+    end.
+
+Definition sum_bimap {A B C D} (f : A -> B) (g : C -> D) :
+  A + C -> B + D :=
+  sum_elim (inl ∘ f) (inr ∘ g).
+
+Definition sum_map_l {A B C} (f : A -> B) : A + C -> B + C :=
+  sum_bimap f id.
+
+Definition sum_map_r {A B C} (f : A -> B) : C + A -> C + B :=
+  sum_bimap id f.
 
 Definition sum_assoc_r {A B C} (abc : (A + B) + C) : A + (B + C) :=
   match abc with
@@ -20,10 +41,10 @@ Definition sum_assoc_r {A B C} (abc : (A + B) + C) : A + (B + C) :=
   | inr c => inr (inr c)
   end.
 
-Definition sum_assoc_l {A B C} (abc : A + (B + C)) : (A + B) + C.
-Admitted.
+Definition sum_comm {A B} : A + B -> B + A :=
+  sum_elim inr inl.
 
-Definition sum_elim {A B C} (f : A -> C) (g : B -> C) : A + B -> C.
+Definition sum_assoc_l {A B C} (abc : A + (B + C)) : (A + B) + C.
 Admitted.
 
 Definition sum_merge {A} : A + A -> A := sum_elim id id.
@@ -59,26 +80,71 @@ Arguments code {A B}.
 Definition den A B : Type := A -> itree E0 B.
 (* den can represent both blocks (A -> block B) and asm (asm A B). *)
 
-Notation eq_den d1 d2 := (forall a, eutt eq (d1 a) (d2 a)).
+Notation eq_den_ d1 d2 := (forall a, eutt eq (d1 a) (d2 a)).
+
+Definition eq_den {E A B} (d1 d2 : A -> itree E B) :=
+  (forall a, eutt eq (d1 a) (d2 a)).
+
+(* Sequential composition of den. *)
+Definition seq_den {A B C} (ab : den A B) (bc : den B C) : den A C :=
+  fun a => ab a >>= bc.
+
+Infix ">=>" := seq_den (at level 40).
+
+Definition id_den {A} : den A A := fun a => Ret a.
+
+Definition lift_den {A B} (f : A -> B) : den A B := fun a => Ret (f a).
+
+Definition den_sum_map_r {A B C} (ab : den A B) : den (C + A) (C + B) :=
+  sum_elim (lift_den inl) (ab >=> lift_den inr).
+
+Definition den_sum_bimap {A B C D} (ab : den A B) (cd : den C D) :
+  den (A + C) (B + D) :=
+  sum_elim (ab >=> lift_den inl) (cd >=> lift_den inr).
 
 (* Denotation of [bks] *)
 Axiom denote_b : forall {A B}, bks A B -> den A B.
 
 (* Denotation of [asm] *)
 Definition denote_asm {A B} : asm A B -> den A B :=
-  fun s a => loop (denote_b (code s)) (inl a).
+  fun s => seq_den (lift_den inl) (loop (denote_b (code s))).
+
+(* A denotation of an asm program can be viewed as a circuit/diagram
+   where wires correspond to jumps/program links.
+
+   A [box : den A (A + B)] is a circuit, drawn below as ###,
+   with one input wire labeled by A, and two output wires labeled
+   by A and B.
+
+   The [loop : den A (A + B) -> den A B] combinator closes the
+   circuit, linking the box with itself by plugging the A output
+   back into the output.
+
+     +-----+
+     | ### |
+  A--+-###-+
+       ###----B
+       ###
+
+ *)
 
 (* Denotation of [cat_b] *)
-Definition cat_den : forall {A B C D},
+Definition cat_den {A B C D} :
     (den A B) ->
     (den C D) ->
-    (den (A + C) (B + D)).
-Admitted.
+    (den (A + C) (B + D)) := den_sum_bimap.
 
 (* Denotation of [rewire_b] *)
 Definition rewire_den {A B C D} (f : C -> A) (g : B -> D)
            (ab : den A B) : den C D :=
   fun a => ITree.map g (ab (f a)).
+
+Lemma unfold_rewire_den {A B C D} (f : C -> A) (g : B -> D)
+      (ab : den A B) :
+  eq_den (rewire_den f g ab)
+         (lift_den f >=> ab >=> lift_den g).
+Proof.
+Admitted.
 
 (* Correctness of [cat_b] and [rewire_b] (easy) *)
 
@@ -118,12 +184,129 @@ Definition seq_bks {A I B J C}
 Definition seq_asm {A B C} (ab : asm A B) (bc : asm B C) : asm A C :=
   {| code := seq_bks (code ab) (code bc) |}.
 
-(* Sequential composition of den. *)
-Definition seq_den {A B C} (ab : den A B) (bc : den B C) : den A C :=
-  fun a => ab a >>= bc.
+(* Unused but should go to FixFacts *)
+Instance eutt_loop {E A B} :
+  Proper ((eq ==> eutt eq) ==> eq ==> eutt eq) (@loop E A B).
+Proof.
+Admitted.
+
+Instance eutt_loop' {E A B} :
+  Proper (eq_den ==> eq_den) (@loop E A B).
+Proof.
+Admitted.
+
+Instance eutt_rewire_den {A B C D} :
+  Proper ((eq ==> eq) ==> (eq ==> eq) ==> eq_den ==> eq_den)
+         (@rewire_den A B C D).
+Proof.
+Admitted.
+
+Instance eutt_seq_den {A B C} :
+  Proper (eq_den ==> eq_den ==> eq_den) (@seq_den A B C).
+Proof.
+Admitted.
+
+Instance Equivalence_eq_den {E A B} : Equivalence (@eq_den E A B).
+Proof.
+Admitted.
+
+Lemma seq_den_assoc {A B C D}
+      (ab : den A B) (bc : den B C) (cd : den C D) :
+  eq_den ((ab >=> bc) >=> cd)
+         (ab >=> (bc >=> cd)).
+Proof.
+Admitted.
+
+Lemma seq_loop_l {A B C}
+      (ab : den A (A + B)) (bc : den B C) :
+  eq_den (loop ab >=> bc)
+         (lift_den inl >=> loop (den_sum_bimap ab bc)).
+Proof.
+Admitted.
+
+Lemma seq_loop_l_seq {A B C}
+      (ab : den A (A + B)) (bc : den B C) :
+  eq_den (loop ab >=> bc)
+         (loop (ab >=> den_sum_map_r bc)).
+Proof.
+Admitted.
+
+(*
+Lemma seq_loop_r {A B C}
+      (ab : den A B) (bc : den B (B + C)) :
+  eq_den (ab >=> loop bc)
+         (loop (
+*)
+
+Instance eutt_elim {E A B C} :
+  Proper (eq_den ==> eq_den ==> eq_den) (@sum_elim A B (itree E C)).
+Proof.
+  repeat intro. destruct a; unfold sum_elim; auto.
+Qed.
+
+(*
+
+loop_loop (f : A -> B) (box : den B (B + (A + C))):
+
+These two loops (where wires represent jumps):
+
+        +------------+
+        |   +-----+  |
+        |   | ### |  |
+        | f-+-###-+B |
+     A--+-+   ###----+A
+              ###-------C
+              ###
+
+Can be rewired as:
+
+            +---------+
+            | ###     |
+          +-+-###--+--+B
+     A----+f  ###--+f    <- A
+              ###------C
+              ###
+
+*)
+Lemma loop_loop {A B C}
+      (f : A -> B) (bc : den B (B + (A + C))) :
+  eq_den (loop (lift_den f >=> loop bc))
+         (lift_den f
+             >=> loop (bc >=> lift_den (sum_elim inl (sum_elim (inl ∘ f) inr)))).
+Proof.
+Admitted.
+
+Lemma sum_elim_loop {A B C BD}
+      (f : B -> BD)
+      (ac : den A C) (bc : den BD (BD + C)) :
+  eq_den (sum_elim ac
+                   (lift_den f >=> loop bc))
+         (lift_den (sum_map_r f)
+            >=> loop (sum_elim (ac >=> lift_den inr)
+                               (bc >=> lift_den (sum_map_l inr)))).
+Proof.
+Admitted.
 
 Theorem seq_correct {A B C} (ab : asm A B) (bc : asm B C) :
   eq_den (denote_asm (seq_asm ab bc))
          (seq_den (denote_asm ab) (denote_asm bc)).
+Proof.
+  unfold denote_asm, seq_asm; simpl.
+  unfold seq_bks.
+  rewrite rewire_correct.
+  rewrite cat_correct.
+  unfold cat_den.
+  rewrite unfold_rewire_den.
+  rewrite (seq_den_assoc (_ inl)).
+  rewrite seq_loop_l.
+  unfold den_sum_bimap.
+  rewrite (seq_den_assoc (_ inl)).
+  rewrite seq_loop_l_seq.
+  unfold den_sum_map_r.
+  rewrite sum_elim_loop.
+  rewrite loop_loop.
+
+Arguments loop : clear implicits.
+
+Qed.
 Admitted.
-(* Use FixFacts.bind_loop to prove this *)
